Source/DafnyLanguageServer/SymbolTable/LanguageServerVisitorBase.cs
@@ -7,6 +7,7 @@ using System.Threading.Tasks;
 using Microsoft.Boogie;
 using Microsoft.Dafny;
 using Serilog.Sinks.File;
+using IdentifierExpr = Microsoft.Dafny.IdentifierExpr;
 using LiteralExpr = Microsoft.Dafny.LiteralExpr;
 using LocalVariable = Microsoft.Dafny.LocalVariable;
 using Type = Microsoft.Dafny.Type;
