Test/LanguageServerTest/DafnyFiles/symbolTable/06_GoTo.dfy
@@ -4,7 +4,7 @@ method MultipleReturns(inp1: int, inp2: int) returns (more: int, less: int)
 {
    more := inp1 + inp2;
    less := inp1 - inp2;
-   assert more == 0;
+   assert more == 0; 
 }
 class ClassA {
    constructor () { }
